src/tc/tcutil.fs
@@ -538,9 +538,13 @@ let lift_assumption env f =
   lift_formula env t_unit assume_pure assume_pure f
 
 let lift_pure env t f = 
-  let assert_pure = must <| Tc.Env.lookup_typ_abbrev env Const.assert_pure_lid in
-  let assume_pure = must <| Tc.Env.lookup_typ_abbrev env Const.assume_pure_lid in
-  lift_formula env t assert_pure assume_pure f
+  let md = Tc.Env.get_monad_decl env Const.pure_effect_lid in
+  let a, kwp = Tc.Env.wp_signature env md.mname in 
+  let k = Util.subst_kind' [Inl(a.v, t)] kwp in
+  let trivial = mk_Typ_app(md.trivial, [targ t]) k f.pos in
+  let wp = mk_Typ_app(md.assert_p, [targ t; targ f; targ trivial]) k f.pos in
+  let wlp = mk_Typ_app(md.assume_p, [targ t; targ f; targ trivial]) k f.pos in
+  mk_comp md t wp wlp []
 
 let refresh_comp_label env b c = 
     if Util.is_ml_comp c then c
@@ -592,44 +596,56 @@ let weaken_precondition env c f = match f with
       let wlp = mk_Typ_app(md.assume_p, [targ res_t; targ f; targ wlp]) wlp.tk wlp.pos in
       mk_comp md res_t wp wlp c.flags
 
-let bind_cases env (res_t:typ) (cases:list<(option<formula> * comp)>) : comp =
+let bind_cases env (res_t:typ) (cases:list<(formula * comp)>) : comp =
   (if List.length cases = 0 then failwith "Empty cases!"); (* TODO: Fix precedence of semi colon *)
-  match cases with 
-    | [(None, c)] -> c
-    | [(Some f, c)] -> strengthen_precondition (Some Errors.exhaustiveness_check) env c (NonTrivial f)
-    | _ -> 
-      let caccum, some_pat_matched = cases |> List.fold_left (fun (caccum, prior_pat_matched) (gopt, c) -> 
-        let prior_or_c_matched, cguard = match prior_pat_matched, gopt with 
-          | None, Some g -> Some g, Some g
-          | Some g, None -> prior_pat_matched, Some <| Util.mk_neg g
-          | Some g, Some g' -> Some (Util.mk_disj g g'), Some <| Util.mk_conj (Util.mk_neg g) g'
-          | None, None -> None, None in
-        let c = match cguard with 
-          | None -> c
-          | Some g -> weaken_precondition env c (NonTrivial g) in 
-        match caccum with 
-          | None -> (Some c, prior_or_c_matched)
-          | Some caccum -> 
-            let (md, a, kwp), (t, wp1, wlp1), (_, wp2, wlp2) = lift_and_destruct env caccum c in 
-            let k = Util.subst_kind' [Inl(a.v, t)] kwp in
-            let wp_conj wp1 wp2 = 
-              mk_Typ_app(md.wp_binop, [targ t; targ wp1; targ (Util.ftv Const.and_lid (Const.kbin ktype ktype ktype)); targ wp2]) k wp2.pos in
-            let wp = wp_conj wp1 wp2 in
-            let wlp = wp_conj wlp1 wlp2 in 
-            (Some <| mk_comp md t wp wlp [], prior_or_c_matched)) (None, None) in
-      let caccum = comp_to_comp_typ <|  (must <| caccum) in
-      let md = Tc.Env.get_monad_decl env caccum.effect_name in
-      let res_t, wp, wlp = destruct_comp caccum in
-      let wp = match some_pat_matched with 
-        | None -> wp 
-        | Some guard ->
-          let guard = label Errors.exhaustiveness_check (Env.get_range env) guard in
-          mk_Typ_app(md.assert_p, [targ res_t; targ guard; targ wp]) wp.tk wp.pos in
-      let a, kwp = Tc.Env.wp_signature env caccum.effect_name in
-      let k = Util.subst_kind' [Inl(a.v, res_t)] kwp in
-      let wp = mk_Typ_app(md.ite_wp, [targ res_t; targ wlp; targ wp]) k wp.pos in
-      let wlp = mk_Typ_app(md.ite_wlp, [targ res_t; targ wlp]) k wlp.pos in
-      mk_comp md res_t wp wlp []
+//  match cases with 
+//    | [(f, c)] -> strengthen_precondition (Some Errors.exhaustiveness_check) env c (NonTrivial f)
+//    | _ -> 
+    let ifthenelse md res_t g wp_t wp_e = mk_Typ_app(md.if_then_else, [targ res_t; targ g; targ wp_t; targ wp_e]) wp_t.tk (Range.union_ranges wp_t.pos wp_e.pos) in
+    let default_case = 
+        lift_pure env res_t (label Errors.exhaustiveness_check (Env.get_range env) (Util.ftv Const.false_lid ktype)) in
+    let comp = List.fold_right (fun (g, cthen) celse ->
+        let (md, a, kwp), (res_t, wp_then, wlp_then), (_, wp_else, wlp_else) = lift_and_destruct env cthen celse in
+       mk_comp md res_t (ifthenelse md res_t g wp_then wp_else) (ifthenelse md res_t g wlp_then wlp_else) []) cases default_case in
+    let comp = comp_to_comp_typ comp in
+    let md = Tc.Env.get_monad_decl env comp.effect_name in
+    let res_t, wp, wlp = destruct_comp comp in
+    let wp = mk_Typ_app(md.ite_wp, [targ res_t; targ wlp; targ wp]) wp.tk wp.pos in
+    let wlp = mk_Typ_app(md.ite_wlp, [targ res_t; targ wlp]) wlp.tk wlp.pos in
+    mk_comp md res_t wp wlp []
+  
+//      let caccum, some_pat_matched = cases |> List.fold_left (fun (caccum, prior_pat_matched) (gopt, c) -> 
+//        let prior_or_c_matched, cguard = match prior_pat_matched, gopt with 
+//          | None, Some g -> Some g, Some g
+//          | Some g, None -> prior_pat_matched, Some <| Util.mk_neg g
+//          | Some g, Some g' -> Some (Util.mk_disj g g'), Some <| Util.mk_conj (Util.mk_neg g) g'
+//          | None, None -> None, None in
+//        let c = match cguard with 
+//          | None -> c
+//          | Some g -> weaken_precondition env c (NonTrivial g) in 
+//        match caccum with 
+//          | None -> (Some c, prior_or_c_matched)
+//          | Some caccum -> 
+//            let (md, a, kwp), (t, wp1, wlp1), (_, wp2, wlp2) = lift_and_destruct env caccum c in 
+//            let k = Util.subst_kind' [Inl(a.v, t)] kwp in
+//            let wp_conj wp1 wp2 = 
+//              mk_Typ_app(md.wp_binop, [targ t; targ wp1; targ (Util.ftv Const.and_lid (Const.kbin ktype ktype ktype)); targ wp2]) k wp2.pos in
+//            let wp = wp_conj wp1 wp2 in
+//            let wlp = wp_conj wlp1 wlp2 in 
+//            (Some <| mk_comp md t wp wlp [], prior_or_c_matched)) (None, None) in
+//      let caccum = comp_to_comp_typ <|  (must <| caccum) in
+//      let md = Tc.Env.get_monad_decl env caccum.effect_name in
+//      let res_t, wp, wlp = destruct_comp caccum in
+//      let wp = match some_pat_matched with 
+//        | None -> wp 
+//        | Some guard ->
+//          let guard = label Errors.exhaustiveness_check (Env.get_range env) guard in
+//          mk_Typ_app(md.assert_p, [targ res_t; targ guard; targ wp]) wp.tk wp.pos in
+//      let a, kwp = Tc.Env.wp_signature env caccum.effect_name in
+//      let k = Util.subst_kind' [Inl(a.v, res_t)] kwp in
+//      let wp = mk_Typ_app(md.ite_wp, [targ res_t; targ wlp; targ wp]) k wp.pos in
+//      let wlp = mk_Typ_app(md.ite_wlp, [targ res_t; targ wlp]) k wlp.pos in
+//      mk_comp md res_t wp wlp []
 
 let close_comp env bindings (c:comp) = 
   if Util.is_ml_comp c then c
